\documentclass[]{article}
\usepackage{amsmath}
\usepackage{amssymb}
%opening
\title{}
\author{}

\begin{document}

\maketitle

\section*{Question 2: Time Series regression test of CAPM for one asset i (3 points)}
Black, Jensen and Scholes (1972) suggest to test the empirical validity of the CAPM by estimating the following LRM: 

\begin{align*}
	r_{it} - r_{ft} &= \alpha_i + \beta_i(r_{mt} - r_{ft}) + u_{it}\\
	z_{it} &= \alpha_i + \beta_i z_{mt} + u_{it}\\
	u_{it}|z_{mt} &\sim iid(0, \omega^2_i)
\end{align*}

\subsection*{(i) Estimate $\hat{\alpha_i}$ and $\hat{\beta_i}$}
NOTE : $\hat{\alpha_i}$ is the Jensenâ€™s alpha, and represents an estimate of the expected return not justified by its exposure to market risk, the only one that matters according to the CAPM.

\begin{align*}
	x_t &= (1, z_{mt}') \\
	X &= [x_1, ..., x_T]' \\
	X'X &= T Sxx\\
	Sxx &= \frac{1}{T}X'X = \left[\begin{array}{cc}
		1 & \bar{z}_m \\
		\bar{z}_m & \frac{1}{T}\sum{z_m^2}
	\end{array}\right] \\	
	Sxx^{-1} &= \left[\begin{array}{cc}
		\frac{1}{T}\sum{z_m^2} & -\bar{z}_m \\
		-\bar{z}_m & 1
	\end{array}\right] = \left[\begin{array}{cc}
	\frac{1}{T}\sum{z_m^2} - \bar{z}_m^2 + \bar{z}_m^2 & -\bar{z}_m \\
	-\bar{z}_m & 1
	\end{array}\right]\\
	 &= \left[\begin{array}{cc}
		\hat{\sigma}_m^2 + \bar{z}_m^2 & -\bar{z}_m \\
		-\bar{z}_m & 1
	\end{array}\right] = \left[\begin{array}{cc}
	1 + \frac{\bar{z}_m^2}{\hat{\sigma}_m^2} & \frac{-\bar{z}_m}{\hat{\sigma}_m^2} \\
	\frac{-\bar{z}_m}{\hat{\sigma}_m^2} & \frac{1}{\hat{\sigma}^2}
	\end{array}\right]\\
	Sxz_i &= X'z_i = \left[\begin{array}{c}
		\bar{z}_i \\
		\frac{1}{T}\sum{z_m z_i}
	\end{array}\right] = \left[\begin{array}{c}
		\bar{z}_i \\
		\frac{1}{T}\sum{z_m z_i} - \bar{z}_m \bar{z}_i + \bar{z}_m \bar{z}_i
	\end{array}\right] = \left[\begin{array}{c}
		\bar{z}_i \\
		\hat{\sigma}_{im} + \bar{z}_m \bar{z}_i 
	\end{array}\right] \\
\end{align*}

Solving for $\hat{\alpha}_i$ and $\hat{\beta}_i$:
\begin{align*}
		Sxx \left[\begin{array}{c}
		\hat{\alpha}_i \\
		\hat{\beta}_i
	\end{array}\right] & = Sxz_i\\
	\left[\begin{array}{cc}
		1 & \bar{z}_m \\
		\bar{z}_m & \frac{1}{n}\sum{z_m^2}
	\end{array}\right] \left[\begin{array}{c}
		\hat{\alpha}_i \\
		\hat{\beta}_i
	\end{array}\right] &= \left[\begin{array}{c}
		\bar{z}_i \\
		\hat{\sigma}_{im} + \bar{z}_m \bar{z}_i 
	\end{array}\right] \\	
	\begin{array}{c}
		(1) \\
		(2)
	\end{array}
	\left[\begin{array}{c}
		\hat{\alpha}_i + \hat{\beta}_i \bar{z}_m \\
		\hat{\alpha}_i \bar{z}_m + \hat{\beta}_i \frac{1}{n}\sum{z_m^2}
	\end{array}\right] &= \left[\begin{array}{c}
		\bar{z}_i \\
		\hat{\sigma}_{im} + \bar{z}_m \bar{z}_i 
	\end{array}\right] \\
\end{align*}

From (1) follows directly: $\hat{\alpha}_i = \bar{z}_i - \hat{\beta}_i \bar{z}_m$. Inserting this into (2) yields:
\begin{align*}
	\hat{\alpha}_i \bar{z}_m + \hat{\beta}_i \frac{1}{n}\sum{z_m^2} &= \hat{\sigma}_{im} + \bar{z}_m \bar{z}_i \\
	(\bar{z}_i - \hat{\beta}_i \bar{z}_m)\bar{z}_m + \hat{\beta}_i \frac{1}{n}\sum{z_m^2} &= \hat{\sigma}_{im} + \bar{z}_m \bar{z}_i \\
	\bar{z}_i \bar{z}_m - \hat{\beta}_i \bar{z}_m^2 + \hat{\beta}_i \frac{1}{n}\sum{z_m^2} &= \hat{\sigma}_{im} + \bar{z}_m \bar{z}_i \\
	- \hat{\beta}_i \bar{z}_m^2 + \hat{\beta}_i \frac{1}{n}\sum{z_m^2} &= \hat{\sigma}_{im}\\
	\hat{\beta}_i  (\frac{1}{n}\sum{z_m^2}-\bar{z}_m^2) &= \hat{\sigma}_{im}\\
	\hat{\beta}_i \hat{\sigma}_{m}^2 &= \hat{\sigma}_{im}\\
	\hat{\beta}_i &=  \frac{\hat{\sigma}_{im}}{\hat{\sigma}_{m}^2}\\
\end{align*}

\subsection*{(ii) Distribution of  $\hat{\alpha}_i$ and $\hat{\beta}_i$}

Expected value of $\hat{\alpha_i}$ and $\hat{\beta_i}$
\begin{align*}
	\hat{\beta} &= \left[\begin{array}{c}
		\hat{\alpha}_i \\
		\hat{\beta}_i
	\end{array}\right] = (X'X)^{-1}X'z_i = (X'X)^{-1}X'(X \beta + u_{it})\\
	E[\hat{\beta}|z_m] &= (X'X)^{-1}X'X \beta + (X'X)^{-1}X'E[u_{it}|z_m]\\
	E[\hat{\beta}|z_m] &= \beta + (X'X)^{-1}X'0, \text{ by assumption } u_i|z_mt \sim iid(0, \omega_i^2)\\
	E[\hat{\beta}|z_m] &= \beta\\
	E\left[\begin{array}{c}
		\hat{\alpha}_i \\
		\hat{\beta}_i
	\end{array}|z_m\right] &= \left[\begin{array}{c}
	\alpha_i \\
	\beta_i
\end{array}\right]
\end{align*}

Variance $\hat{\alpha}_i$ and $\hat{\beta}_i$
\begin{align*}
	\hat{\beta} &= \left[\begin{array}{c}
		\hat{\alpha}_i \\
		\hat{\beta}_i
	\end{array}\right]\\
	V(\hat{\beta}|z_m) &= V((\hat{\beta} - \beta)|z_m) \text{ (given $\beta$ non-random)}\\
	&= V((X'X)^{-1}X'u_{i}|z_m) = A V(u_{i}|z_m)A' \text{ (with $A=(X'X)^{-1}X'$)}\\
	&= A E[u_{i}^2|z_m] A' = A \omega_i^2A' \text{ by assumption } u_i|z_mt \sim iid(0, \omega_i^2)\\
	&= \omega_i^2AA' = \omega_i^2(X'X)^{-1}X'((X'X)^{-1}X')' = \omega_i^2(X'X)^{-1}X'X(X'X)^{-1}\\
	&= \omega_i^2 (X'X)^{-1} = \omega_i^2 \frac{1}{T}Sxx^{-1}\\
	&= \frac{\omega_i^2}{T}Sxx^{-1} = \frac{\omega_i^2}{T} \left[\begin{array}{cc}
		1 + \frac{\bar{z}_m^2}{\hat{\sigma}_m^2} & \frac{-\bar{z}_m}{\hat{\sigma}_m^2} \\
		\frac{-\bar{z}_m}{\hat{\sigma}_m^2} & \frac{1}{\hat{\sigma}^2}
	\end{array}\right]
\end{align*}

Therefore

\begin{align*}
	\left[\begin{array}{c}
		\hat{\alpha}_i \\
		\hat{\beta}_i
	\end{array}\right] | z_m &\sim N\left(
		\left[\begin{array}{c}
			\alpha_i \\
			\beta_i
		\end{array}\right], 
		\frac{\omega_i^2}{T} \left[\begin{array}{cc}
			1 + \frac{\bar{z}_m^2}{\hat{\sigma}_m^2} & \frac{-\bar{z}_m}{\hat{\sigma}_m^2} \\
			\frac{-\bar{z}_m}{\hat{\sigma}_m^2} & \frac{1}{\hat{\sigma}^2}
		\end{array}\right]
	\right) \square
\end{align*}

\subsection*{(iii) Determine the t-statistics to test $H_0: \beta_{k=1} = \alpha_i = 0$}

Analog to (ii) and replacing the unknown true $\omega_i$ with the sample $\hat{\omega}_i$ obtained from the OLS residuals
\begin{align*}
	V((\hat{\beta} - \beta)|z_m) &= \hat{\omega}_i^2 (X'X)^{-1} = \hat{\omega}_i^2 \frac{1}{T}Sxx^{-1}\\
	V((\hat{\beta}_{k=1} - 0)|z_m) &= \omega_i^2 (X'X)_{kk}^{-1} = \hat{\omega}_i^2 \frac{1}{T}Sxx_{kk}^{-1}\\
	&=  \frac{\hat{\omega}_i^2}{T}(1+\frac{\bar{z}_m^2}{\hat{\sigma}_m^2})\\
	SE((\hat{\beta} - \beta)|z_m) &= \hat{\omega}_i[(1+\frac{\bar{z}_m^2}{\hat{\sigma}_m^2})/T]^{1/2}
\end{align*}

The t-statistic to test $H_0: \beta_{k=1} = \alpha_i = 0$ therefore is : $$ \xi_i = \frac{\hat{\alpha}_i - 0}{\hat{\omega}_i[(1+\frac{\bar{z}_m^2}{\hat{\sigma}_m^2})/T]^{1/2}}  \xrightarrow{d}  N(0,1)$$

\end{document}
